fixing the combination of quantifier pulling and cancellation
- it isn't complete by any means.

MirrorCharge!/src/CancellerTac.v
@@ -2,6 +2,7 @@ Require Import ExtLib.Core.RelDec.
 Require Import ExtLib.Tactics.
 Require Import MirrorCore.SymI.
 Require Import MirrorCore.EnvI.
+Require Import MirrorCore.RawSubst2.
 Require Import MirrorCore.Ext.Expr.
 Require Import MirrorCore.Ext.ExprUnifySyntactic.
 Require Import MirrorCore.Ext.FMapSubst.
@@ -78,13 +79,21 @@ Section ordered_cancel_tac.
     red. inversion 1.
   Qed.
 
-  Definition the_canceller (sls : SepLogSpec func) tus tvs (lhs rhs : expr func) s :=
+  Definition the_canceller (sls : SepLogSpec func) tus tvs (lhs rhs : expr func)
+             (s : subst)
+  : expr func * expr func * list_subst (expr func) :=
     let lhs_norm := normalize sls lhs tus tvs in
     let rhs_norm := normalize sls rhs tus tvs in
     let '(lhs',rhs',s') :=
         ordered_cancel (doUnifySepLog 100 tus tvs) eprovePure
                        (simple_order (func:=func)) lhs_norm rhs_norm s
-    in (conjunctives_to_expr SSL lhs', conjunctives_to_expr SSL rhs', s').
+    in (conjunctives_to_expr SSL lhs',
+        conjunctives_to_expr SSL rhs',
+        @to_list_subst (expr func) subst {| Subst2.lookup := @Subst.lookup _ _ Subst_subst
+                                          ; Subst2.domain :=
+                                            fun m =>
+                                              List.map (@fst _ _) (@FMapSubst.MAP.elements _ (FMapSubst.SUBST.env m))
+                                          |} s').
 
   Variable sls : SepLogSpec func.
   Hypothesis slsOk : @SepLogSpecOk ts _ _ tySL sls _ _.
@@ -108,15 +117,17 @@ Section ordered_cancel_tac.
   Local Instance PureOp_pure : @Pure.PureOp (typD ts nil tySL) := slsOk.(_PureOp).
   Local Instance Pure_pure : @Pure.Pure (typD ts nil tySL) _ _ _ := slsOk.(_Pure).
 
+  Existing Instance Subst_list_subst.
+  Existing Instance SubstOk_list_subst.
+
   Theorem the_cancellerOk (Pure_true : Pure.pure ltrue)
-  : forall us vs lhs rhs lhs' rhs' sub,
+  : forall (us vs : env (typD ts)) lhs rhs lhs' rhs' sub,
       the_canceller sls (typeof_env us) (typeof_env vs) lhs rhs (@FMapSubst.SUBST.subst_empty _) = (lhs', rhs', sub) ->
       match exprD us vs lhs' tySL
           , exprD us vs rhs' tySL
       with
         | Some lhs , Some rhs =>
-          Subst.substD us vs sub /\
-            lhs |-- rhs
+          fold_left and (Subst2.substD us vs sub) (lhs |-- rhs)
         | None , None => True
         | _ , _ => False
       end ->
@@ -179,10 +190,10 @@ Section ordered_cancel_tac.
     { apply split_env_projT2_join_env. auto. }
     assert (vs = join_env h0).
     { apply split_env_projT2_join_env. auto. }
+    rewrite <- H14 in *.
     rewrite <- H15 in *.
-    rewrite <- H16 in *.
     forward_reason.
-    rewrite H6. rewrite H9. assumption.
+    rewrite H6. rewrite H9. admit.
   Qed.
 End ordered_cancel_tac.
 
@@ -564,18 +575,22 @@ Definition canceller_pre
            (FM : fun_map ts) (LM : logic_ops ts) (EM : embed_ops ts)
            (tySL : typ)
            (ILogicOps_SL : ILogicOps (typD ts nil tySL))
-           us vs lhs' rhs' sub : Prop :=
+           us vs lhs' rhs'
+           (sub : list_subst (expr ilfunc)) : Prop :=
   let rsym := @RSym_ilfunc ts FM LM EM in
   match @exprD typ (typD ts) (expr ilfunc) (Expr_expr rsym) us vs lhs' tySL with
     | Some lhs0 =>
       match @exprD typ (typD ts) (expr ilfunc) (Expr_expr rsym) us vs rhs' tySL with
         | Some rhs0 =>
-          @Subst.substD
-            (FMapSubst.SUBST.subst ilfunc) (expr ilfunc) typ (typD ts)
-            (Expr_expr rsym)
-            (FMapSubst.SUBST.Subst_subst _)
-            (FMapSubst.SUBST.SubstOk_subst _) us vs sub
-          /\ (lhs0 |-- rhs0)
+          fold_left and
+                    (@Subst2.substD
+                       (list_subst (expr ilfunc)) typ (typD ts)
+                       (expr ilfunc)
+                       (Expr_expr rsym)
+                       (RawSubst2.Subst_list_subst _)
+                       (RawSubst2.SubstOk_list_subst _) us vs sub)
+                    (lhs0 |-- rhs0)
+                    
         | None => False
       end
     | None =>
@@ -603,7 +618,7 @@ Theorem apply_the_canceller
         (CSL : ConcreteSepLog)
         (CSLok : @ConcreteSepLogOk ts FM LM EM tySL BILO CSL)
 : forall (us vs : env (typD ts)) (lhs rhs lhs' rhs' : expr ilfunc)
-         (sub : SUBST.subst ilfunc),
+         (sub : list_subst (expr ilfunc)),
     the_canceller (@RSym_func ts FM LM EM) tySL
                   (@SynSepLog_ConcreteSepLog_smart tySL CSL)
                   (@SepLogSpec_ConcreteSepLog CSL)
@@ -621,186 +636,3 @@ Proof.
   Grab Existential Variables.
   eapply CSLok.
 Qed.
-
-
-(** THIS IS OLD
-Module SepLogBuilder2.
-  Require Import ILogicFunc.
-
-  Variable ts : types.
-  Let func := ilfunc.
-  Variable RSym_func : RSym (typD ts) func.
-
-  Record ConcreteSepLog : Type :=
-  { ctor_star : func ; ctor_emp : func }.
-
-  Variable (tySL : typ).
-  Variable (OPS : ILogicOps (typD ts nil tySL)).
-  Variable (BILO : BILOperators (typD ts nil tySL)).
-
-  Record ConcreteSepLogOk tySL
-
-         (CSL : ConcreteSepLog) : Type :=
-  { starOk : forall us tvs,
-    exprD' us tvs (Inj CSL.(ctor_star)) (tyArr tySL (tyArr tySL tySL)) =
-    Some (fun _ => sepSP)
-  ; empOk : forall us tvs,
-    exprD' us tvs (Inj CSL.(ctor_emp)) tySL = Some (fun _ => empSP)
-  ; trueOk : forall us tvs,
-    exprD' us tvs (Inj (ilf_true tySL)) = Some (fun _ => ltrue)
-  }.
-
-  Definition func_eq : func -> func -> bool :=
-    RelDec.rel_dec (equ := @eq ilfunc).
-
-  (** NOTE: My [ILogic] must come form LM **)
-  Variable (csl : @ConcreteSepLog tySL BILO).
-  Variable (cslOk : @ConcreteSepLogOk tySL BILO csl).
-
-  Variable PureOp : @Pure.PureOp (typD ts nil tySL).
-  Variable PureLaws : @Pure.Pure _ OPS BILO PureOp.
-
-  Definition SepLogSpec_ConcreteSepLog : SepLogSpec func :=
-  {| is_pure := fun _ => false
-   ; is_emp := func_eq csl.(ctor_emp)
-   ; is_star := func_eq csl.(ctor_star)
-  |}.
-
-  Theorem SepLogSpecOk_ConcreteSepLog
-  : @SepLogSpecOk ts _ RSym_func tySL SepLogSpec_ConcreteSepLog OPS BILO.
-  Proof.
-    refine (@Build_SepLogSpecOk _ _ _ _ _ _ _ PureOp PureLaws _ _ _).
-    abstract (inversion 1).
-    abstract (simpl; intros; unfold func_eq in H;
-              consider (RelDec.rel_dec (equ := @eq ilfunc) (ctor_emp csl) e);
-              intros; subst;
-              unfold exprD; destruct (split_env vs);
-              rewrite (cslOk.(empOk) us x); reflexivity).
-    abstract (simpl; intros; unfold func_eq in H;
-              consider (RelDec.rel_dec (equ := @eq ilfunc) (ctor_star csl) e);
-              intros; subst;
-              unfold exprD; destruct (split_env vs);
-              rewrite (cslOk.(starOk) us x); reflexivity).
-  Defined.
-
-  Definition SynSepLog_ConcreteSepLog : SynSepLog ilfunc :=
-  {| e_star := fun (a b : expr ilfunc) => App (App (Inj csl.(ctor_star)) a) b
-   ; e_emp := Inj csl.(ctor_emp)
-   ; e_true := Inj (ilf_true tySL)
-   ; e_and := fun (a b : expr ilfunc) => App (App (Inj (ilf_and tySL)) a) b
-   |}.
-
-  Hypothesis LMok : logic_opsOk LM.
-
-  Local Instance ILogic_OPS : @ILogic _ OPS.
-  Proof.
-    specialize (LMok tySL).
-    rewrite LM_OPS in LMok. assumption.
-  Defined.
-
-  Lemma typeof_star : typeof_sym (ctor_star csl) = Some (tyArr tySL (tyArr tySL tySL)).
-  Proof.
-    generalize (cslOk.(starOk) nil nil).
-    red_exprD.
-    generalize dependent (symD (ctor_star csl)).
-    forward. inv_all; subst. reflexivity.
-  Qed.
-
-  Theorem typ_eqb_complete : forall x, typ_eqb x x = true.
-  Proof.
-    clear. induction x; simpl; Cases.rewrite_all_goal; auto.
-    { match goal with
-        | |- ?X = _ => consider X
-      end; auto. }
-    { match goal with
-        | |- ?X = _ => consider X
-      end; auto. }
-  Qed.
-
-  Theorem SynSepLogOk_ConcreteSepLog
-  : @SynSepLogOk ts ilfunc _ tySL OPS BILO SynSepLog_ConcreteSepLog.
-  Proof.
-    constructor; simpl; intros.
-    { eexists. split. apply (cslOk.(empOk) us tvs).
-      intros. reflexivity. }
-    { red_exprD.
-      simpl.
-      rewrite LM_OPS.
-      rewrite typ_cast_typ_refl.
-      eexists; split; eauto. simpl. reflexivity. }
-    { generalize (cslOk.(starOk) us tvs).
-      red_exprD. intros.
-      forward. inv_all; subst.
-      exists (fun g => sepSP (valx g) (valy g)).
-      split; [ | intros; reflexivity ].
-      generalize typeof_star. simpl. intro.
-      rewrite H3. simpl.
-      rewrite exprD'_type_cast in H.
-      rewrite exprD'_type_cast in H0.
-      forward.
-      repeat match goal with
-               | H : ?X = _ |- context [ ?Y ] =>
-                 change Y with X ; rewrite H
-             end.
-      inv_all; subst.
-      rewrite typ_eqb_complete.
-      red_exprD.
-      rewrite H3.
-      red_exprD.
-      rewrite H1.
-      repeat match goal with
-               | H : ?X = _ |- context [ ?Y ] =>
-                 change Y with X ; rewrite H
-             end.
-      f_equal.
-      change (let K := (fun x g => (x g) (t3 g) (t1 g)) in
-              K (fun _ : HList.hlist (typD ts nil) tvs => t) =
-              K (fun _ : HList.hlist (typD ts nil) tvs => sepSP)).
-      intro. clearbody K. f_equal. auto. }
-    { generalize (cslOk.(starOk) us tvs); intros.
-      red_exprD.
-      forward. inv_all; subst.
-      generalize dependent (symD (ctor_star csl)).
-      rewrite typeof_star.
-      simpl. rewrite typ_cast_typ_refl.
-      intros. inv_all; subst.
-      red_exprD.
-      forward. inv_all; subst.
-      simpl in H8.
-      forward. inv_all; subst.
-      assert (t6 = tySL /\ t1 = tySL).
-      { generalize typeof_star. simpl.
-        intro. rewrite H in *.
-        inv_all. auto. }
-      destruct H; subst.
-      do 2 eexists. split; eauto. split; eauto.
-      rewrite cslOk.(starOk) in H3. inv_all. subst.
-      reflexivity. }
-    { red_exprD.
-      rewrite LM_OPS.
-      rewrite exprD'_type_cast in H.
-      forward. inv_all; subst.
-      simpl.
-      rewrite typ_eqb_complete.
-      red_exprD.
-      rewrite LM_OPS.
-      red_exprD.
-      rewrite LM_OPS.
-      rewrite typ_cast_typ_refl.
-      rewrite H2. rewrite H0. eexists; split; eauto.
-      simpl. reflexivity. }
-    { red_exprD.
-      rewrite LM_OPS in H.
-      forward. inv_all; subst.
-      red_exprD.
-      rewrite LM_OPS in H1.
-      forward. inv_all; subst.
-      red_exprD.
-      simpl in *; rewrite LM_OPS in H.
-      forward. inv_all. subst t4 t0 t t2 p.
-      do 2 eexists; split; eauto. split; eauto.
-      intros.
-      uip_all. reflexivity. }
-  Qed.
-End SepLogBuilder.
-**)
