MirrorCharge!/src/QuantCancel.v
@@ -1,59 +1,169 @@
-Require Import ILogic ILInsts.
-Require Import ILogicFunc.
-Require Import MirrorCore.Ext.Types.
-Require Import MirrorCore.Ext.ExprCore.
+Require Import ExtLib.Tactics.
 Require Import MapPositive.
 Require Import MirrorCore.SymI.
-Require Import ExtLib.Core.RelDec.
-Require Import Coq.Bool.Bool.
-Require Import ExtLib.Data.Positive.
-Require Import Ext.ExprLift.
-Require Import ExtLib.Tactics.Consider.
+Require Import MirrorCore.EnvI.
+Require Import MirrorCore.Ext.Types.
+Require Import MirrorCore.Ext.ExprCore.
+Require Import MirrorCore.Ext.ExprLift.
 Require Import MirrorCore.Ext.Expr.
 Require Import MirrorCore.Ext.ExprD.
 Require Import MirrorCore.Ext.ExprTactics.
-Require Import MirrorCore.EnvI.
-Require Import ExtLib.Tactics.Cases.
-Require Import ExtLib.Tactics.Injection.
-Require Import ExtLib.Tactics.EqDep.
-Require Import Ext.SetoidFold.
-Require Import Relation_Definitions.
 Require Import MirrorCore.Ext.AppFull.
-Require Import ILFFold SepLogFold. 
+Require Import MirrorCore.Ext.SetoidFold.
+(** Charge **)
+Require Import ILogic ILInsts.
+(** MirrorCharge **)
+Require Import ILogicFunc.
+Require Import ILFFold SepLogFold.
 Require Import ILPullQuantStar.
 Require Import CancellerTac.
 Require Import SynSepLog.
 
 Section QuantCancel.
-	Context (ts : types) (funcs : fun_map ts).
+    Context (ts : types) (funcs : fun_map ts).
     Context (gs : logic_ops ts) {gsOk : logic_opsOk gs}.
     Context {es : embed_ops ts} {esOk : embed_opsOk gs es}.
-    
+
     Variable slspec : SepLogSpec ilfunc.
     Variable synsl : SynSepLog ilfunc.
-    
+
     Variable ltyp : typ.
-    
+
     Definition subst := FMapSubst.SUBST.subst ilfunc.
 
     Local Instance RSym_sym : SymI.RSym (typD ts) ilfunc := RSym_ilfunc funcs gs es.
 
-    
     Definition lift_uvars {func : Type} : nat -> nat -> expr func -> expr func := fun _ _ p => p.
 
-	Definition pull_exists := @app_fold (option (list typ * expr ilfunc)) pq_var pq_uvar pq_inj pq_abs (pq_app slspec) pq_exists pq_forall.
+    Definition pull_exists :=
+      @app_fold (option (list typ * expr ilfunc))
+                pq_var pq_uvar pq_inj pq_abs (pq_app slspec) pq_exists pq_forall.
 
-	Definition qcancel (tus tvs : tenv typ) (P Q : expr ilfunc) : option (expr ilfunc * expr ilfunc * subst) :=
-	    match pull_exists Q tus tvs with
-	    	| Some (xs, Q') => 
-	    	    let P' := lift_uvars (length tus) (length xs) P in
-	    		let Q'' := vars_to_uvars (length tus) 0 (length xs) Q' in
-	    		Some (@the_canceller ts ilfunc _ ltyp synsl slspec (tus++xs) tvs P' Q'' (FMapSubst.SUBST.subst_empty _))
-	    	| None => None
-	    end.
-	    
-	   (* 
-	    P 5 ** Q |-- Q ** exists y, P y.
-	*)
+    Record CancelResult : Type :=
+    { NewExs : tenv typ
+    ; Subst  : RawSubst2.list_subst (expr ilfunc)
+    ; Lhs    : expr ilfunc
+    ; Rhs    : expr ilfunc
+    }.
+
+    Definition qcancel (tus tvs : tenv typ) (P Q : expr ilfunc)
+    : option CancelResult :=
+      match pull_exists Q tus tvs with
+	| Some (xs, Q') =>
+	  let P' := lift_uvars (length tus) (length xs) P in
+	  let Q'' := vars_to_uvars (length tus) 0 (length xs) Q' in
+	  let '(lhs, rhs, s') :=
+              @the_canceller ts ilfunc _ ltyp synsl slspec (tus++xs) tvs
+                             P' Q'' (FMapSubst.SUBST.subst_empty _)
+          in Some {| NewExs := xs ; Lhs := lhs ; Rhs := rhs ; Subst := s' |}
+	| None => None
+      end.
+
 End QuantCancel.
-	
+
+(** TODO: We're shadowing notation somewhere? **)
+Require Import ILogic.
+Require Import BILogic.
+
+Definition canceller_post
+           (ts : types)
+           (FM : fun_map ts) (LM : logic_ops ts) (EM : embed_ops ts)
+           (tySL : typ)
+           (ILogicOps_SL : ILogicOps (typD ts nil tySL))
+           us vs lhs rhs : Prop :=
+  let rsym := @RSym_ilfunc ts FM LM EM in
+  match @exprD typ (typD ts) (expr ilfunc) (Expr_expr rsym) us vs lhs tySL with
+    | Some lhs0 =>
+      match @exprD typ (typD ts) (expr ilfunc) (Expr_expr rsym) us vs rhs tySL with
+        | Some rhs0 => lhs0 |-- rhs0
+        | None => True
+      end
+    | None => True
+  end.
+
+Section existsAll.
+  Variable ts : types.
+
+  Fixpoint existsAll (tvs : tenv typ) : (HList.hlist (typD ts nil) tvs -> Prop) -> Prop :=
+    match tvs as tvs return (HList.hlist (typD ts nil) tvs -> Prop) -> Prop with
+      | nil => fun k => k (@HList.Hnil _ _)
+      | tv :: tvs => fun k =>
+        exists x : typD ts nil tv,
+          existsAll tvs (fun g => k (HList.Hcons x g))
+    end.
+End existsAll.
+
+Check @ExprI.exprD'.
+
+Definition canceller_pre
+           (ts : types)
+           (FM : fun_map ts) (LM : logic_ops ts) (EM : embed_ops ts)
+           (tySL : typ)
+           (ILogicOps_SL : ILogicOps (typD ts nil tySL))
+           us vs (res : CancelResult) : Prop :=
+  let rsym := @RSym_ilfunc ts FM LM EM in
+  let E := Expr_expr rsym in
+  match res with
+    | {| NewExs := texs ; Lhs := lhs' ; Rhs := rhs' ; Subst := sub |} =>
+      let (tus,us) := split_env us in
+      let (tvs,vs') := split_env vs in
+      match
+        @ExprI.exprD' _ _ _ E (tus ++ texs) tvs lhs' tySL with
+        | Some lhs' =>
+          match @ExprI.exprD' _ _ _ E (tus ++ texs) tvs rhs' tySL with
+            | Some rhs' =>
+              existsAll ts texs (fun us' =>
+                let us := HList.hlist_app us us' in
+                fold_right and
+                           (lhs' us vs' |-- rhs' us vs')
+                           (@Subst2.substD
+                              (RawSubst2.list_subst (expr ilfunc)) typ (typD ts)
+                              (expr ilfunc)
+                              (Expr_expr rsym)
+                              (RawSubst2.Subst_list_subst _)
+                              (RawSubst2.SubstOk_list_subst _) (join_env us) vs sub))
+            | None => False
+          end
+        | None =>
+          match @ExprI.exprD' _ _ _ E (tus ++ texs) tvs rhs' tySL with
+            | Some _ => False
+            | None => True
+          end
+      end
+  end.
+
+Theorem apply_the_canceller
+        (ts : types)
+        (FM : fun_map ts) (LM : logic_ops ts) (EM : embed_ops ts)
+        (LMok : logic_opsOk LM) (EMok : embed_opsOk LM EM)
+        (tySL : typ)
+        (ILogicOps_SL : ILogicOps (typD ts nil tySL))
+        (pf : LM tySL = Some ILogicOps_SL)
+        (BILO : BILOperators (typD ts nil tySL))
+        (BIL : BILogic (typD ts nil tySL))
+        (PureOp : @Pure.PureOp (typD ts nil tySL))
+        (PureLaws : @Pure.Pure _ ILogicOps_SL BILO PureOp)
+        (Hpuretrue : Pure.pure ltrue)
+        (CSL : ConcreteSepLog)
+        (CSLok : @ConcreteSepLogOk ts FM LM EM tySL BILO CSL)
+: forall (us vs : env (typD ts)) (lhs rhs : expr ilfunc) result,
+    @qcancel ts FM LM EM
+                  (@SepLogSpec_ConcreteSepLog CSL)
+                  (@SynSepLog_ConcreteSepLog_smart tySL CSL)
+                  tySL
+                  (typeof_env us) (typeof_env vs) lhs rhs =
+    Some result ->
+    @canceller_pre ts FM LM EM tySL ILogicOps_SL us vs result ->
+    @canceller_post ts FM LM EM tySL ILogicOps_SL us vs lhs rhs.
+Proof.
+(*  intros.
+  eapply the_cancellerOk in H; eauto with typeclass_instances.
+  { eapply SynSepLogOk_ConcreteSepLog_smart; eauto. }
+  { unfold SepLogSpec_ConcreteSepLog.
+    instantiate (1 := @SepLogSpecOk_ConcreteSepLog _ _ _ _ _ _ _ _ _ _ _).
+    eapply Hpuretrue. }
+  Grab Existential Variables.
+  eapply CSLok. (** TODO: This is sketchy! **)
+Qed.
+*)
+Admitted.
